exercises/chapter05-distributed-state-machines/exercise03.dfy
@@ -16,14 +16,62 @@ module TwoPCInvariantProof {
     requires v.WF()
   {
     // FIXME: fill in here (solution: 5 lines)
-     true // Replace me
-    // END EDIT
+    && (CommitMsg(Commit) in v.network.sentMsgs ==> CoordinatorVars(v).decision == Some(Commit))
+    && (CommitMsg(Abort) in v.network.sentMsgs ==> CoordinatorVars(v).decision == Some(Abort))
+       // END EDIT
   }
 
   // We use this block of code to define additional invariants. We recommend you
   // define predicates for the individual parts of your invariant, to make
   // debugging easier.
   // FIXME: fill in here (solution: 20 lines)
+
+  // 1. the decision of participant implies commit message sent
+  ghost predicate ParticipantRecordDecision(v: Variables)
+    requires v.WF()
+  {
+    && (forall i : nat |
+          && ValidParticipantId(v, i)
+          && ParticipantVars(v, i).decision == Some(Commit)
+          :: CommitMsg(Commit) in v.network.sentMsgs)
+    && (forall i : nat |
+          && ValidParticipantId(v, i)
+          && ParticipantVars(v, i).decision == Some(Abort)
+          :: CommitMsg(Abort) in v.network.sentMsgs)
+  }
+
+  // 2. commit message sent the decision of the coordinator
+  // See DecisionMsgsAgreeWithDecision
+
+  // 3.the decision of the coordinator implies the record of the votes
+  ghost predicate CoordinatorMakesDecision(v: Variables)
+    requires v.WF()
+  {
+    && (CoordinatorVars(v).decision == Some(Commit) ==>
+          forall i : nat | ValidParticipantId(v, i) ::
+            CoordinatorVars(v).votes[i] == Some(Yes))
+    && (CoordinatorVars(v).decision == Some(Abort) ==>
+          exists i : nat | ValidParticipantId(v, i) ::
+            CoordinatorVars(v).votes[i] == Some(No))
+  }
+
+  // 4. the record of the votes implies the vote message sent
+  ghost predicate CoordinatorRecordsVotes(v: Variables)
+    requires v.WF()
+  {
+    forall i : nat | ValidParticipantId(v, i) ::
+      && (CoordinatorVars(v).votes[i] == Some(Yes) ==> VoteMsg(i, Yes) in v.network.sentMsgs)
+      && (CoordinatorVars(v).votes[i] == Some(No) ==> VoteMsg(i, No) in v.network.sentMsgs)
+  }
+
+  // 5. the vote message sent implies the preference of the participant
+  ghost predicate ParticipantSendVote(v: Variables)
+    requires v.WF()
+  {
+    forall i : nat | ValidParticipantId(v, i) ::
+      && (VoteMsg(i, Yes) in v.network.sentMsgs ==> ParticipantVars(v, i).c.preference == Yes)
+      && (VoteMsg(i, No) in v.network.sentMsgs ==> ParticipantVars(v, i).c.preference == No)
+  }
   // END EDIT
 
 
@@ -31,7 +79,10 @@ module TwoPCInvariantProof {
   {
     && v.WF()
        // FIXME: fill in here (solution: 2 lines)
-       // END EDIT
+    && CoordinatorMakesDecision(v)
+    && CoordinatorRecordsVotes(v)
+    && ParticipantSendVote(v)
+    && ParticipantRecordDecision(v)
        // We give you the blueprint for one invariant to get you started...
     && DecisionMsgsAgreeWithDecision(v)
        // ...but you'll need more.
@@ -43,6 +94,14 @@ module TwoPCInvariantProof {
     ensures Inv(v)
   {
     // FIXME: fill in here (solution: 3 lines)
+    assert CoordinatorMakesDecision(v);
+    assert CoordinatorRecordsVotes(v);
+    assert ParticipantSendVote(v);
+    assert ParticipantRecordDecision(v);
+    assert DecisionMsgsAgreeWithDecision(v);
+    assert SafetyAC1(v);
+    assert SafetyAC3(v);
+    assert SafetyAC4(v);
     // END EDIT
   }
 
@@ -53,6 +112,49 @@ module TwoPCInvariantProof {
   {
     //(not all of the below but much of it)
     // FIXME: fill in here (solution: 59 lines)
+    assert ParticipantSendVote(v');
+    assert CoordinatorRecordsVotes(v');
+    assert CoordinatorMakesDecision(v');
+    assert DecisionMsgsAgreeWithDecision(v');
+    assert ParticipantRecordDecision(v');
+
+
+    forall i : HostId |
+      && ValidParticipantId(v', i)
+      && ParticipantVars(v', i).decision != None
+      ensures ParticipantVars(v', i).decision == CoordinatorVars(v').decision
+    {
+      match ParticipantVars(v', i).decision {
+        case Some(Commit) => {
+          assert ParticipantVars(v', i).c.preference == Yes;
+          assert CoordinatorVars(v').votes[i] == Some(Yes);
+          assert CoordinatorVars(v').decision == Some(Commit);
+        }
+        case Some(Abort) => {
+          assert CommitMsg(Abort) in v'.network.sentMsgs;
+          assert CoordinatorVars(v').decision == Some(Abort);
+        }
+      }
+    }
+    assert SafetyAC1(v');
+
+    assert SafetyAC3(v');
+
+    match CoordinatorVars(v').decision {
+      case Some(Commit) => {
+        assert CoordinatorVars(v').decision == Some(Commit);
+        assert SafetyAC4(v');
+      }
+      case Some(Abort) => {
+        assert CoordinatorVars(v').decision == Some(Abort);
+        assert exists i : HostId | ValidParticipantId(v', i) :: CoordinatorVars(v').votes[i] == Some(No);
+        assert SafetyAC4(v');
+      }
+      case None => {
+        assert CoordinatorVars(v').decision == None;
+        assert SafetyAC4(v');
+      }
+    }
     // END EDIT
   }
 
